aneris/aneris_lang/state_interp/state_interp_socket_interp_coh.v
@@ -26,206 +26,280 @@ Section state_interpretation.
   Proof. intros Hall Hin. specialize (Hall sag Hin). by apply set_choose_L. Qed.
 
   (* socket_interp_coh *)
-  Lemma socket_interp_coh_init ips C A M σ f :
-    dom M = A →
-    dom (state_ports_in_use σ) = ips →
-    A ⊆ C →
-    (∀ ip, ip ∈ ips → state_ports_in_use σ !! ip = Some ∅) →
-    (∀ sag sa, sag ∈ A → sa ∈ sag → ip_of_address sa ∈ ips) →
-    set_Forall is_singleton (C ∖ A) →
-    ([∗ set] sag ∈ A, sag ⤇* f sag)%I -∗
+  Lemma socket_interp_coh_init C :
     socket_address_group_ctx C -∗
-    fixed_groups A -∗
-    saved_si_auth M -∗
-    socket_interp_coh (state_ports_in_use σ).
+    unfixed_groups_auth C -∗
+    saved_si_auth ∅ -∗
+    socket_interp_coh.
   Proof.
-    iIntros (<- <- HAle Hpiiu Hfixdom Hsingleton) "? Hctx ? ?".
-    rewrite /socket_interp_coh.
-    iDestruct (socket_address_group_ctx_valid with "Hctx") as %[_ Hne].
-    iExists _, _, _; iFrame.
-    iSplit.
-    { iExists _. iFrame. iSplit; [ eauto | ].
-      iApply (big_sepS_mono with "[$]"); auto. }
-    iSplit; [done|]. iSplit; [done|].
-    iPureIntro. intros sag. split; auto.
-    intros [Hb | [Hb [Hdisj HP]]]; [done|].
-    destruct HP as (sa & ps & Hsain & Hlookup & Hpsin).
-    assert (ip_of_address sa ∈ dom (state_ports_in_use σ)) as Hdom.
-    { apply elem_of_dom. eexists _. apply Hlookup. }
-    specialize (Hpiiu (ip_of_address sa) Hdom).
-    rewrite Hlookup in Hpiiu.
-    assert (ps = ∅) by naive_solver; subst. done.
+    iIntros "Hsags Hunfixed Hsis".
+    iExists _, _. iFrame. iSplit; [done|].
+    rewrite difference_diag_L.
+    iExists _.
+    iFrame. iSplit; [by iPureIntro; set_solver|done].
   Qed.
 
-  Lemma socket_interp_coh_fixed_valid sag A ips :
-    sag ∈ A →
-    socket_interp_coh ips -∗ fixed_groups A -∗ ∃ φ, sag ⤇* φ.
+  (* (* socket_interp_coh *) *)
+  (* Lemma socket_interp_coh_init ips C A M σ f : *)
+  (*   dom M = A → *)
+  (*   dom (state_ports_in_use σ) = ips → *)
+  (*   A ⊆ C → *)
+  (*   (∀ ip, ip ∈ ips → state_ports_in_use σ !! ip = Some ∅) → *)
+  (*   (∀ sag sa, sag ∈ A → sa ∈ sag → ip_of_address sa ∈ ips) → *)
+  (*   set_Forall is_singleton (C ∖ A) → *)
+  (*   ([∗ set] sag ∈ A, sag ⤇* f sag)%I -∗ *)
+  (*   socket_address_group_ctx C -∗ *)
+  (*   unfixed_groups A -∗ *)
+  (*   saved_si_auth M -∗ *)
+  (*   socket_interp_coh (state_ports_in_use σ). *)
+  (* Proof. *)
+  (*   iIntros (<- <- HAle Hpiiu Hfixdom Hsingleton) "? Hctx ? ?". *)
+  (*   rewrite /socket_interp_coh. *)
+  (*   iDestruct (socket_address_group_ctx_valid with "Hctx") as %[_ Hne]. *)
+  (*   iExists _, _, _; iFrame. *)
+  (*   iSplit. *)
+  (*   { iExists _. iFrame. iSplit; [ eauto | ]. *)
+  (*     iApply (big_sepS_mono with "[$]"); auto. } *)
+  (*   iSplit; [done|]. iSplit; [done|]. *)
+  (*   iPureIntro. intros sag. split; auto. *)
+  (*   intros [Hb | [Hb [Hdisj HP]]]; [done|]. *)
+  (*   destruct HP as (sa & ps & Hsain & Hlookup & Hpsin). *)
+  (*   assert (ip_of_address sa ∈ dom (state_ports_in_use σ)) as Hdom. *)
+  (*   { apply elem_of_dom. eexists _. apply Hlookup. } *)
+  (*   specialize (Hpiiu (ip_of_address sa) Hdom). *)
+  (*   rewrite Hlookup in Hpiiu. *)
+  (*   assert (ps = ∅) by naive_solver; subst. done. *)
+  (* Qed. *)
+
+  (* Lemma socket_interp_coh_fixed_valid sag A ips : *)
+  (*   sag ∈ A → *)
+  (*   socket_interp_coh ips -∗ fixed_groups A -∗ ∃ φ, sag ⤇* φ. *)
+  (* Proof. *)
+  (*   iIntros (HaA) "Hscoh #HA". *)
+  (*   iDestruct "Hscoh" as (sags sis A') "(Hctx & HA' & Hsiauth & %Hle & %Hsingle & %Hdom)". *)
+  (*   iDestruct (fixed_agree with "HA HA'") as %<-. *)
+  (*   iDestruct (socket_address_group_ctx_valid with "Hctx") as %[_ Hin]. *)
+  (*   assert (sag ∈ sags) as Hasags by set_solver. *)
+  (*   pose proof (set_choose_forall_L _ _ Hin Hasags) as [sa Hsa]. *)
+  (*   iDestruct ("Hsiauth") as (sis') "(Hsiauth & <- & Hsis)". *)
+  (*   iDestruct (big_sepS_elem_of with "Hsis") as "$". *)
+  (*   erewrite Hdom; eauto. *)
+  (* Qed. *)
+
+  (* Lemma unfixed_update_dealloc' A B : *)
+  (*   ⊢ unfixed_groups_auth A ∗ unfixed_groups B ==∗ *)
+  (*     unfixed_groups_auth (A ∖ B). *)
+  (* Proof. Admitted. *)
+
+
+  Lemma socket_address_group_own_subseteq `{anerisG Mdl}
+        (sags sags' : gset socket_address_group) :
+    sags' ⊆ sags →
+    socket_address_groups_own sags -∗
+    socket_address_groups_own sags'.
   Proof.
-    iIntros (HaA) "Hscoh #HA".
-    iDestruct "Hscoh" as (sags sis A') "(Hctx & HA' & Hsiauth & %Hle & %Hsingle & %Hdom)".
-    iDestruct (fixed_agree with "HA HA'") as %<-.
-    iDestruct (socket_address_group_ctx_valid with "Hctx") as %[_ Hin].
-    assert (sag ∈ sags) as Hasags by set_solver.
-    pose proof (set_choose_forall_L _ _ Hin Hasags) as [sa Hsa].
-    iDestruct ("Hsiauth") as (sis') "(Hsiauth & <- & Hsis)".
-    iDestruct (big_sepS_elem_of with "Hsis") as "$".
-    erewrite Hdom; eauto.
+    iIntros (Hle) "Hsags".
+    rewrite /socket_address_groups_own.
+    apply subseteq_disjoint_union_L in Hle.
+    destruct Hle as [Z [-> Hdisj]].
+    setoid_rewrite <-disj_gsets_op_union.
+    iDestruct "Hsags" as "[H1 H2]".
+    iFrame.
   Qed.
 
-  Lemma socket_interp_coh_socketbind_static ps P sa sag A :
-    sa ∈ sag →
-    sag ∈ A →
-    P !! ip_of_address sa = Some ps →
-    port_of_address sa ∉ ps →
-    fixed_groups A -∗
-    socket_interp_coh P -∗
-    socket_interp_coh (<[ip_of_address sa:={[port_of_address sa]} ∪ ps]> P).
+  Lemma set_lemma `{Countable A} (X Y Z : gset A) :
+    Z ⊆ Y → Y ⊆ X → X ∖ Y ∪ Z = X ∖ (Y ∖ Z).
+  Proof. Admitted.
+
+  Lemma socket_interp_coh_allocate sag φ :
+    socket_interp_coh -∗
+    unfixed_groups {[sag]} ==∗
+    sag ⤇* φ ∗ socket_interp_coh.
   Proof.
-    iIntros (?? Hpsin ?) "HA". rewrite /socket_interp_coh.
-    iDestruct 1 as (sags sis A') "(Hown & HA' & Hsiauth & %Hle & %Hsingle & %Hdms)".
-    iDestruct (fixed_agree with "HA HA'") as %<-.
-    iDestruct (socket_address_group_ctx_valid with "Hown") as %[Hdisj Hne].
-    pose proof (socket_interp_coh_le _ _ _ Hdms) as Hle'.
-    pose proof (all_disjoint_subseteq _ _ Hle Hdisj) as HdisjA.
-    iExists _,_,_. iFrame. iPureIntro.
-    split; [done|]. split; [done|].
-    intros sag'. rewrite Hdms.
-    split; intros [|(Hnin & Helems & sa' & ps' & Hin & HPlookup & Hpsin')]; auto.
-    { right. split; [done|]. split; [done|].
-      destruct (decide (ip_of_address sa = ip_of_address sa')) as [Heq|].
-      - eexists _, _. split; [done|]. rewrite Heq lookup_insert. split; [done|].
-        rewrite -Heq Hpsin in HPlookup.
-        assert (ps = ps') by naive_solver; subst.
-        by apply elem_of_union_r.
-      - eexists _, _. by rewrite lookup_insert_ne //. }
-    destruct (decide (ip_of_address sa = ip_of_address sa')) as [Heq|].
-    { rewrite Heq lookup_insert in HPlookup.
-      assert ({[port_of_address sa]} ∪ ps = ps') as <- by naive_solver.
-      apply elem_of_union in Hpsin'.
-      destruct Hpsin' as [Hdm%elem_of_singleton_1 | Hdm].
-      - destruct sa, sa'; simpl in *. simplify_eq.
-        assert ((SocketAddressInet address0 port) ∈
-                ({[SocketAddressInet address0 port]}:gset _))
-          as Hin by set_solver.
-        assert (all_disjoint ({[{[SocketAddressInet address0 port]}]} ∪ A)).
-        { apply (all_disjoint_union {[{[SocketAddressInet address0 port]}]} A).
-          split.
-          { by apply all_disjoint_singleton. }
-          split.
-          { eapply all_disjoint_subseteq. done. done. }
-          done. }
-        assert (sag = {[SocketAddressInet address0 port]}).
-        { eapply (elem_of_all_disjoint_eq _ _ _ _); set_solver. }
-        naive_solver.
-      - right. split; [done|]. split; [done|]. eexists _, _. split; [done|].
-        split; [by rewrite -Heq|].
-        done. }
-    right. split; [done|]. split; [done|].
-    eexists _, _. split; [done|].
-    rewrite lookup_insert_ne in HPlookup; done.
+    iIntros "Hinterp Hsag".
+    iDestruct "Hinterp" as (sags A Hle) "(Hsags & Hunfixed & Hsis)".
+    iAssert (⌜sag ∈ A⌝)%I as %Hin.
+    { iDestruct (own_valid_2 with "Hunfixed Hsag") as %Hvalid.
+      rewrite auth_both_valid_discrete in Hvalid.
+      destruct Hvalid as [Hincluded Hvalid].
+      rewrite gset_disj_included in Hincluded.
+      iPureIntro. set_solver. }    
+    iAssert (socket_address_group_own sag) as "#Hsag'".
+    { rewrite /socket_address_group_own.
+      iApply (socket_address_group_own_subseteq sags); [set_solver|].
+      by iApply socket_address_groups_ctx_own. }    
+    iMod (unfixed_update_dealloc with "[$Hunfixed $Hsag]") as "Hunfixed".
+    iDestruct "Hsis" as (sis) "(Hsaved & %Hdom & Hsis)".
+    iMod (socket_interp_alloc with "Hsag' Hsaved")
+      as (γsi) "[Hsaved #Hsi]".
+    { apply not_elem_of_dom. set_solver. }
+    iModIntro. iFrame "#∗".
+    iExists sags, (A ∖ {[sag]}).
+    iSplit; [iPureIntro; set_solver|].
+    iFrame. iExists _. iSplit; [done|].    
+    iSplit; [iPureIntro|].
+    { rewrite dom_insert_L.
+      rewrite Hdom. rewrite -set_lemma; [set_solver|set_solver|done]. }
+    rewrite -set_lemma; [|set_solver|done].
+    iApply big_sepS_union; [set_solver|].
+    iFrame. iApply big_sepS_singleton.
+    iExists _. iFrame "#".
   Qed.
 
-  Lemma socket_interp_coh_socketbind_dynamic ps P sa A φ :
-    sa ∉ ⋃ₛ A →
-    P !! ip_of_address sa = Some ps →
-    port_of_address sa ∉ ps →
-    fixed_groups A -∗
-    socket_interp_coh P ==∗
-    socket_interp_coh (<[ip_of_address sa:={[port_of_address sa]} ∪ ps]> P) ∗
-    sa ⤇1 φ.
-  Proof.
-    iIntros (? Hpa Hps) "#HA". rewrite /socket_interp_coh.
-    iDestruct 1 as (sags sis A') "(Hctx & HA' & Hsiauth & %Hle & %Hsingle & %Hdms)".
-    iDestruct ("Hsiauth") as (sis') "(Hsiauth & <- & #Hsis)".
-    iDestruct (fixed_agree with "HA HA'") as %<-.
-    iDestruct (socket_address_group_ctx_valid with "Hctx") as %[Hdisj Hne].
-    pose proof (socket_interp_coh_le _ _ _ Hdms) as Hle'.
-    pose proof (all_disjoint_subseteq _ _ Hle Hdisj) as Hdisj_sis.
-    pose proof (all_disjoint_subseteq _ _ Hle' Hdisj_sis) as HdisjA.
-    assert (sis' !! {[sa]} = None).
-    { destruct (sis' !! {[sa]}) eqn:Heq; last done.
-      destruct (Hdms {[sa]}) as [[Hin |] _]; [ by eapply elem_of_dom_2 | | ].
-      - assert (sa ∈ ({[sa]}:socket_address_group)) as Hin' by set_solver.
-        pose proof (elem_of_union_set_mono _ _ _ Hin Hin') as Hin''.
-        contradiction.
-      - by set_solver. }
-    iDestruct (socket_address_group_ctx_valid with "Hctx") as %[_ Hall].
-    iMod (socket_address_group_ctx_update _ {[{[sa]}]} with "Hctx") as "[Hctx Hown]".
-    { apply all_disjoint_singleton. }
-    { destruct (decide ({[sa]} ∈ sags)).
-      { by apply have_disj_elems_elem_of. }
-      apply have_disj_elems_singleton.
-      intros x Hx.
-      right.
-      assert (sa ∉ ⋃ₛ sags).
-      { assert ({[sa]} ∉ sags ∖ A).
-        { apply not_elem_of_difference. left. done. }
-        eapply not_elem_of_union_set_difference; [done|].
-        intros Hsa. apply H1.
-        by apply elem_of_union_set_singletons. }
-      pose proof (set_choose_forall_L x _ Hall Hx) as [x' Hxin].
-      pose proof (elem_of_union_set_mono _ _ _ Hx Hxin) as Hx'.
-      symmetry.
-      intros x'' Hx1 Hx2.
-      assert (x'' = sa) by set_solver; simplify_eq.
-      pose proof (elem_of_union_set_mono _ _ _ Hx Hx1).
-      set_solver. }
-    { apply set_Forall_singleton. rewrite /is_ne. set_solver. }
-    iMod (socket_interp_alloc {[sa]} φ sis' with "Hown Hsiauth")
-      as (?) "[Hsiauth #Hφ]"; [done|].
-    iFrame "Hφ". iModIntro.
-    iExists _, _, _; iFrame.
-    iSplitL "Hsis Hsiauth".
-    { iExists _.
-      iFrame.
-      rewrite dom_insert_L.
-      iSplit; [done|].
-      rewrite big_sepS_insert; last rewrite not_elem_of_dom //.
-      iFrame "#".
-      iExists _. iFrame "Hφ". }
-    iSplit; [iPureIntro;set_solver|].
-    iSplit.
-    { iPureIntro.
-      assert ({[sa]} ∉ A).
-      { by apply not_elem_of_union_set_singleton. }
-      assert (({[{[sa]}]} ∪ sags) ∖ A = {[{[sa]}]} ∪ (sags ∖ A)) as Heq.
-      { set_solver. }
-      rewrite Heq.
-      apply set_Forall_union; [|done].
-      apply set_Forall_singleton. rewrite /is_singleton. by eauto. }
-    iIntros (sag).
-    iPureIntro.
-    rewrite elem_of_union elem_of_singleton Hdms.
-    split.
-    - intros [->| Hdom].
-      + right.
-        split; [ by apply not_elem_of_union_set_singleton |].
-        pose proof (all_disjoint_have_disj_elems_singleton A sa HdisjA H).
-        split; [done|].
-        eexists _, _.
-        split; [done|]. rewrite lookup_insert. split; [done|].
-        by apply elem_of_union_l, elem_of_singleton.
-      + destruct Hdom as [? | (Hnin & Helems & sa' & ps' & -> & HPlookup & Hpsin')];
-          [by left|].
-        right. split; [done|].
-        destruct (decide (ip_of_address sa = ip_of_address sa')) as [Heq |Hneq].
-        * split; [done|]. eexists _, _. split; [done|].
-          destruct Heq. rewrite lookup_insert. intros; simplify_eq.
-          split; [done|]. by apply elem_of_union_r.
-        * split; [done|]. eexists _, _. by rewrite lookup_insert_ne.
-    - intros [Hin | (Hnin & Helems & sa' & ps' & -> & HPlookup & Hpsin')]; [by auto|].
-      destruct (decide (sa = sa')) as [Heq | Hneq]; [ by left; f_equiv | ].
-      right; right. split; [done|].
-      destruct (decide (ip_of_address sa = ip_of_address sa')) as [Heq|].
-      + split; [done|]. eexists _, _.
-        rewrite Heq lookup_insert in HPlookup. split; [done|].
-        rewrite -Heq. split; [eauto|].
-        assert ({[port_of_address sa]} ∪ ps = ps') by naive_solver; subst.
-        apply elem_of_union in Hpsin'. destruct Hpsin' as [Hpsin' | Hport].
-        * apply elem_of_singleton_1 in Hpsin'.
-          destruct sa,sa'; simpl in *; simplify_eq.
-        * intros. destruct Heq; simplify_eq; eauto.
-      + split; [done|]. intros. eexists _, _. by rewrite lookup_insert_ne in HPlookup.
-  Qed.
+  (* Lemma socket_interp_coh_socketbind_static ps P sa sag A : *)
+  (*   sa ∈ sag → *)
+  (*   sag ∈ A → *)
+  (*   P !! ip_of_address sa = Some ps → *)
+  (*   port_of_address sa ∉ ps → *)
+  (*   fixed_groups A -∗ *)
+  (*   socket_interp_coh P -∗ *)
+  (*   socket_interp_coh (<[ip_of_address sa:={[port_of_address sa]} ∪ ps]> P). *)
+  (* Proof. *)
+  (*   iIntros (?? Hpsin ?) "HA". rewrite /socket_interp_coh. *)
+  (*   iDestruct 1 as (sags sis A') "(Hown & HA' & Hsiauth & %Hle & %Hsingle & %Hdms)". *)
+  (*   iDestruct (fixed_agree with "HA HA'") as %<-. *)
+  (*   iDestruct (socket_address_group_ctx_valid with "Hown") as %[Hdisj Hne]. *)
+  (*   pose proof (socket_interp_coh_le _ _ _ Hdms) as Hle'. *)
+  (*   pose proof (all_disjoint_subseteq _ _ Hle Hdisj) as HdisjA. *)
+  (*   iExists _,_,_. iFrame. iPureIntro. *)
+  (*   split; [done|]. split; [done|]. *)
+  (*   intros sag'. rewrite Hdms. *)
+  (*   split; intros [|(Hnin & Helems & sa' & ps' & Hin & HPlookup & Hpsin')]; auto. *)
+  (*   { right. split; [done|]. split; [done|]. *)
+  (*     destruct (decide (ip_of_address sa = ip_of_address sa')) as [Heq|]. *)
+  (*     - eexists _, _. split; [done|]. rewrite Heq lookup_insert. split; [done|]. *)
+  (*       rewrite -Heq Hpsin in HPlookup. *)
+  (*       assert (ps = ps') by naive_solver; subst. *)
+  (*       by apply elem_of_union_r. *)
+  (*     - eexists _, _. by rewrite lookup_insert_ne //. } *)
+  (*   destruct (decide (ip_of_address sa = ip_of_address sa')) as [Heq|]. *)
+  (*   { rewrite Heq lookup_insert in HPlookup. *)
+  (*     assert ({[port_of_address sa]} ∪ ps = ps') as <- by naive_solver. *)
+  (*     apply elem_of_union in Hpsin'. *)
+  (*     destruct Hpsin' as [Hdm%elem_of_singleton_1 | Hdm]. *)
+  (*     - destruct sa, sa'; simpl in *. simplify_eq. *)
+  (*       assert ((SocketAddressInet address0 port) ∈ *)
+  (*               ({[SocketAddressInet address0 port]}:gset _)) *)
+  (*         as Hin by set_solver. *)
+  (*       assert (all_disjoint ({[{[SocketAddressInet address0 port]}]} ∪ A)). *)
+  (*       { apply (all_disjoint_union {[{[SocketAddressInet address0 port]}]} A). *)
+  (*         split. *)
+  (*         { by apply all_disjoint_singleton. } *)
+  (*         split. *)
+  (*         { eapply all_disjoint_subseteq. done. done. } *)
+  (*         done. } *)
+  (*       assert (sag = {[SocketAddressInet address0 port]}). *)
+  (*       { eapply (elem_of_all_disjoint_eq _ _ _ _); set_solver. } *)
+  (*       naive_solver. *)
+  (*     - right. split; [done|]. split; [done|]. eexists _, _. split; [done|]. *)
+  (*       split; [by rewrite -Heq|]. *)
+  (*       done. } *)
+  (*   right. split; [done|]. split; [done|]. *)
+  (*   eexists _, _. split; [done|]. *)
+  (*   rewrite lookup_insert_ne in HPlookup; done. *)
+  (* Qed. *)
+
+  (* Lemma socket_interp_coh_socketbind_dynamic ps P sa A φ : *)
+  (*   sa ∉ ⋃ₛ A → *)
+  (*   P !! ip_of_address sa = Some ps → *)
+  (*   port_of_address sa ∉ ps → *)
+  (*   fixed_groups A -∗ *)
+  (*   socket_interp_coh P ==∗ *)
+  (*   socket_interp_coh (<[ip_of_address sa:={[port_of_address sa]} ∪ ps]> P) ∗ *)
+  (*   sa ⤇1 φ. *)
+  (* Proof. *)
+  (*   iIntros (? Hpa Hps) "#HA". rewrite /socket_interp_coh. *)
+  (*   iDestruct 1 as (sags sis A') "(Hctx & HA' & Hsiauth & %Hle & %Hsingle & %Hdms)". *)
+  (*   iDestruct ("Hsiauth") as (sis') "(Hsiauth & <- & #Hsis)". *)
+  (*   iDestruct (fixed_agree with "HA HA'") as %<-. *)
+  (*   iDestruct (socket_address_group_ctx_valid with "Hctx") as %[Hdisj Hne]. *)
+  (*   pose proof (socket_interp_coh_le _ _ _ Hdms) as Hle'. *)
+  (*   pose proof (all_disjoint_subseteq _ _ Hle Hdisj) as Hdisj_sis. *)
+  (*   pose proof (all_disjoint_subseteq _ _ Hle' Hdisj_sis) as HdisjA. *)
+  (*   assert (sis' !! {[sa]} = None). *)
+  (*   { destruct (sis' !! {[sa]}) eqn:Heq; last done. *)
+  (*     destruct (Hdms {[sa]}) as [[Hin |] _]; [ by eapply elem_of_dom_2 | | ]. *)
+  (*     - assert (sa ∈ ({[sa]}:socket_address_group)) as Hin' by set_solver. *)
+  (*       pose proof (elem_of_union_set_mono _ _ _ Hin Hin') as Hin''. *)
+  (*       contradiction. *)
+  (*     - by set_solver. } *)
+  (*   iDestruct (socket_address_group_ctx_valid with "Hctx") as %[_ Hall]. *)
+  (*   iMod (socket_address_group_ctx_update _ {[{[sa]}]} with "Hctx") as "[Hctx Hown]". *)
+  (*   { apply all_disjoint_singleton. } *)
+  (*   { destruct (decide ({[sa]} ∈ sags)). *)
+  (*     { by apply have_disj_elems_elem_of. } *)
+  (*     apply have_disj_elems_singleton. *)
+  (*     intros x Hx. *)
+  (*     right. *)
+  (*     assert (sa ∉ ⋃ₛ sags). *)
+  (*     { assert ({[sa]} ∉ sags ∖ A). *)
+  (*       { apply not_elem_of_difference. left. done. } *)
+  (*       eapply not_elem_of_union_set_difference; [done|]. *)
+  (*       intros Hsa. apply H1. *)
+  (*       by apply elem_of_union_set_singletons. } *)
+  (*     pose proof (set_choose_forall_L x _ Hall Hx) as [x' Hxin]. *)
+  (*     pose proof (elem_of_union_set_mono _ _ _ Hx Hxin) as Hx'. *)
+  (*     symmetry. *)
+  (*     intros x'' Hx1 Hx2. *)
+  (*     assert (x'' = sa) by set_solver; simplify_eq. *)
+  (*     pose proof (elem_of_union_set_mono _ _ _ Hx Hx1). *)
+  (*     set_solver. } *)
+  (*   { apply set_Forall_singleton. rewrite /is_ne. set_solver. } *)
+  (*   iMod (socket_interp_alloc {[sa]} φ sis' with "Hown Hsiauth") *)
+  (*     as (?) "[Hsiauth #Hφ]"; [done|]. *)
+  (*   iFrame "Hφ". iModIntro. *)
+  (*   iExists _, _, _; iFrame. *)
+  (*   iSplitL "Hsis Hsiauth". *)
+  (*   { iExists _. *)
+  (*     iFrame. *)
+  (*     rewrite dom_insert_L. *)
+  (*     iSplit; [done|]. *)
+  (*     rewrite big_sepS_insert; last rewrite not_elem_of_dom //. *)
+  (*     iFrame "#". *)
+  (*     iExists _. iFrame "Hφ". } *)
+  (*   iSplit; [iPureIntro;set_solver|]. *)
+  (*   iSplit. *)
+  (*   { iPureIntro. *)
+  (*     assert ({[sa]} ∉ A). *)
+  (*     { by apply not_elem_of_union_set_singleton. } *)
+  (*     assert (({[{[sa]}]} ∪ sags) ∖ A = {[{[sa]}]} ∪ (sags ∖ A)) as Heq. *)
+  (*     { set_solver. } *)
+  (*     rewrite Heq. *)
+  (*     apply set_Forall_union; [|done]. *)
+  (*     apply set_Forall_singleton. rewrite /is_singleton. by eauto. } *)
+  (*   iIntros (sag). *)
+  (*   iPureIntro. *)
+  (*   rewrite elem_of_union elem_of_singleton Hdms. *)
+  (*   split. *)
+  (*   - intros [->| Hdom]. *)
+  (*     + right. *)
+  (*       split; [ by apply not_elem_of_union_set_singleton |]. *)
+  (*       pose proof (all_disjoint_have_disj_elems_singleton A sa HdisjA H). *)
+  (*       split; [done|]. *)
+  (*       eexists _, _. *)
+  (*       split; [done|]. rewrite lookup_insert. split; [done|]. *)
+  (*       by apply elem_of_union_l, elem_of_singleton. *)
+  (*     + destruct Hdom as [? | (Hnin & Helems & sa' & ps' & -> & HPlookup & Hpsin')]; *)
+  (*         [by left|]. *)
+  (*       right. split; [done|]. *)
+  (*       destruct (decide (ip_of_address sa = ip_of_address sa')) as [Heq |Hneq]. *)
+  (*       * split; [done|]. eexists _, _. split; [done|]. *)
+  (*         destruct Heq. rewrite lookup_insert. intros; simplify_eq. *)
+  (*         split; [done|]. by apply elem_of_union_r. *)
+  (*       * split; [done|]. eexists _, _. by rewrite lookup_insert_ne. *)
+  (*   - intros [Hin | (Hnin & Helems & sa' & ps' & -> & HPlookup & Hpsin')]; [by auto|]. *)
+  (*     destruct (decide (sa = sa')) as [Heq | Hneq]; [ by left; f_equiv | ]. *)
+  (*     right; right. split; [done|]. *)
+  (*     destruct (decide (ip_of_address sa = ip_of_address sa')) as [Heq|]. *)
+  (*     + split; [done|]. eexists _, _. *)
+  (*       rewrite Heq lookup_insert in HPlookup. split; [done|]. *)
+  (*       rewrite -Heq. split; [eauto|]. *)
+  (*       assert ({[port_of_address sa]} ∪ ps = ps') by naive_solver; subst. *)
+  (*       apply elem_of_union in Hpsin'. destruct Hpsin' as [Hpsin' | Hport]. *)
+  (*       * apply elem_of_singleton_1 in Hpsin'. *)
+  (*         destruct sa,sa'; simpl in *; simplify_eq. *)
+  (*       * intros. destruct Heq; simplify_eq; eauto. *)
+  (*     + split; [done|]. intros. eexists _, _. by rewrite lookup_insert_ne in HPlookup. *)
+  (* Qed. *)
 
 End state_interpretation.
